adapted bd typing to never recheck contexts

pcuic/theories/bidirectional/BDEnvironmentTyping.v
@@ -4,6 +4,8 @@ From MetaCoq.Template Require Import config utils BasicAst AstUtils
 From MetaCoq.PCUIC Require Import PCUICAst PCUICTyping.
 From Equations Require Import Equations.
 
+Require Import ssreflect.
+
 (** Variation on lift_typing to enable a different predicate for checking a body and infering a sort when there is no body *)
 Definition lift_sorting
   (checking : global_env_ext -> context -> term -> term -> Type)
@@ -14,6 +16,112 @@ Definition lift_sorting
     | Some T => checking Σ Γ t T
     | None => { s : Universe.t & sorting Σ Γ t s }
     end.
+
+  Section All_local_env_rel.
+
+  Definition All_local_rel P Γ Γ'
+    := (All_local_env (fun Γ0 t T => P (Γ ,,, Γ0) t T) Γ').
+
+  Definition All_local_rel_nil {P Γ} : All_local_rel P Γ []
+    := localenv_nil.
+
+  Definition All_local_rel_abs {P Γ Γ' A na} :
+    All_local_rel P Γ Γ' -> P (Γ ,,, Γ') A None
+    -> All_local_rel P Γ (Γ',, vass na A)
+    := localenv_cons_abs.
+
+  Definition All_local_rel_def {P Γ Γ' t A na} :
+    All_local_rel P Γ Γ' ->
+    P (Γ ,,, Γ') A None ->
+    P (Γ ,,, Γ') t (Some A) ->
+    All_local_rel P Γ (Γ',, vdef na t A)
+    := localenv_cons_def.
+
+  Lemma All_local_rel_local :
+    forall P Γ,
+      All_local_env P Γ ->
+      All_local_rel P [] Γ.
+  Proof.
+    intros P Γ h. eapply All_local_env_impl.
+    - exact h.
+    - intros Δ t [] h'.
+      all: cbn.
+      + rewrite app_context_nil_l. assumption.
+      + rewrite app_context_nil_l. assumption.
+  Defined.
+
+  Lemma All_local_local_rel P Γ :
+    All_local_rel P [] Γ -> All_local_env P Γ.
+  Proof.
+    intro X. eapply All_local_env_impl. exact X.
+    intros Γ0 t [] XX; cbn in XX; rewrite app_context_nil_l in XX; assumption.
+  Defined.
+
+  Lemma All_local_app_rel {P Γ Γ'} :
+    All_local_env P (Γ ,,, Γ') -> All_local_env P Γ × All_local_rel P Γ Γ'.
+  Proof.
+    induction Γ'.
+    - intros hΓ.
+      split.
+      1: exact hΓ.
+      constructor.
+    - inversion 1 ; subst.
+      all: edestruct IHΓ' ; auto.
+      all: split ; auto.
+      all: constructor ; auto.
+  Defined.
+
+  Lemma All_local_rel_app {P Γ Γ'} :
+    All_local_env P Γ -> All_local_rel P Γ Γ' -> All_local_env P (Γ ,,, Γ').
+  Proof.
+    intros ? hΓ'.
+    induction hΓ'.
+    - assumption.
+    - cbn.
+      constructor ; auto.
+    - cbn.
+      constructor ; auto.
+  Defined.
+
+End All_local_env_rel.
+
+Section All_local_env_size.
+
+  Context (P : context -> term -> option term -> Type) (Psize : forall Γ t T, P Γ t T -> size).
+
+  Fixpoint All_local_env_size Γ (w : All_local_env P Γ) : size :=
+    match w with
+    | localenv_nil => 1
+    | localenv_cons_abs Γ' na t w' p => Psize _ _ _ p + All_local_env_size _ w'
+    | localenv_cons_def Γ' na b t w' pt pb => Psize _ _ _ pt + Psize _ _ _ pb + All_local_env_size _ w'
+    end.
+
+  Lemma All_local_env_size_pos Γ w : 0 < All_local_env_size Γ w.
+  Proof.
+    induction w.
+    all: simpl ; lia.
+  Qed.
+
+End All_local_env_size.
+
+Lemma All_local_env_size_app P Psize Γ Γ' (wfΓ : All_local_env P Γ) (wfΓ' : All_local_rel P Γ Γ') :
+  All_local_env_size _ Psize _ (All_local_rel_app wfΓ wfΓ') + 1 = All_local_env_size _ Psize _ wfΓ + All_local_env_size _ (fun Δ => Psize (Γ,,,Δ)) _ wfΓ'.
+Proof.
+  induction Γ'.
+  - dependent inversion wfΓ'.
+    reflexivity.
+  - revert IHΓ'.
+    dependent inversion wfΓ' ; subst ; intros.
+    + cbn.
+      etransitivity.
+      2: rewrite Nat.add_comm -Nat.add_assoc [X in _ + X]Nat.add_comm -IHΓ' Nat.add_assoc ; reflexivity.
+      reflexivity.
+    + cbn.
+      etransitivity.
+      2: rewrite Nat.add_comm -Nat.add_assoc [X in _ + X]Nat.add_comm -IHΓ' Nat.add_assoc ; reflexivity.
+      reflexivity.
+Qed. 
+      
 
 Section SortingEnv.
 
@@ -61,18 +169,15 @@ Section SortingEnv.
     Context (ssize : forall (Σ : global_env_ext) (Γ : context) (t : term) (u : Universe.t), sorting Σ Γ t u -> size).
     Context (Σ : global_env_ext).
 
-    Fixpoint All_local_env_sorting_size Γ (w : All_local_env (lift_sorting checking sorting Σ) Γ) : size :=
-      match w with
-      | localenv_nil => 1
-      | localenv_cons_abs Γ na t wfΓ h => ssize _ _ _ _ h.π2 + All_local_env_sorting_size _ wfΓ
-      | localenv_cons_def Γ na b t wfΓ ht hb => ssize _ _ _ _ ht.π2 + csize _ _ _ _ hb + All_local_env_sorting_size _ wfΓ
-      end.
-
-    Lemma All_local_env_sorting_size_pos Γ w : 0 < All_local_env_sorting_size Γ w.
+    Definition lift_sorting_size Γ t T (w : lift_sorting checking sorting Σ Γ t T) : size.
     Proof.
-      induction w.
-      all: simpl ; lia.
-    Qed.
+      destruct T.
+      - exact (csize _ _ _ _ w).
+      - exact (ssize _ _ _ _ w.π2).
+    Defined.
+
+    Definition All_local_env_sorting_size := All_local_env_size _ lift_sorting_size.
+    Definition All_local_rel_sorting_size Γ Γ' (wfΓ' : All_local_rel (lift_sorting checking sorting Σ) Γ Γ') := All_local_env_size _ (fun Δ => lift_sorting_size (Γ ,,, Δ)) Γ' wfΓ'.
 
   End All_local_env_size.
 
